Which of the following formulas are equivalent?
\begin{enumerate}[label=(\alph*)]
    \item $P \rightarrow (Q \rightarrow R)$.
    \item $Q \rightarrow (P \rightarrow R)$.
    \item $(P \rightarrow Q) \wedge (P \rightarrow R)$.
    \item $(P \wedge Q) \rightarrow R$.
    \item $P \rightarrow (Q \wedge R)$.
\end{enumerate}


\textbf{Solution:}
\begin{enumerate}[label=(\alph*)]
    \item We show that $P \rightarrow (Q \rightarrow R) \equiv (P \wedge Q) \rightarrow R$. 
    \begin{alignat*}{2}
        P \rightarrow (Q \rightarrow R) &\equiv \neg P \vee (Q \rightarrow R) && \quad \textbf{Conditional Law}\\
        &\equiv \neg P \vee (\neg Q \vee R) && \quad \textbf{Conditional Law}\\
        &\equiv (\neg P \vee \neg Q) \vee R && \quad \textbf{Associative Law}\\
        &\equiv \neg (P \wedge Q) \vee R && \quad \textbf{DeMorgan's Law}\\
        &\equiv (P \wedge Q) \rightarrow R && \quad \textbf{Conditional Law}\\
    \end{alignat*}
    \item We show that $Q \rightarrow (P \rightarrow R) \equiv (P \wedge Q) \rightarrow R$.
    \begin{alignat*}{2}
        Q \rightarrow (P \rightarrow R) &\equiv \neg Q \vee (P \rightarrow R) && \quad \textbf{Conditional Law}\\
        &\equiv \neg Q \vee (\neg P \vee R) && \quad \textbf{Conditional Law}\\
        &\equiv (\neg Q \vee \neg P) \vee R && \quad \textbf{Associative Law}\\
        &\equiv \neg (Q \wedge P) \vee R && \quad \textbf{DeMorgan's Law}\\
        &\equiv \neg (P \wedge Q) \vee R && \quad \textbf{Commutative Law}\\
        &\equiv (P \wedge Q) \rightarrow R && \quad \textbf{Conditional Laws}\\
    \end{alignat*}
    \item We show that $(P \rightarrow Q) \wedge (P \rightarrow R) \equiv P \rightarrow (Q \wedge R)$ by \textbf{Lemma 7.a.2}.
    \item $(P \wedge Q) \rightarrow R$.
    \item $P \rightarrow (Q \wedge R)$.
\end{enumerate}
We conclude that by noting that exercises \textbf{10a, 10b, 10d} are all equivalent. \\
And exercises \textbf{10c, 10e} are equivalent.