Use the laws stated in the text to find simpler formulas equivalent to these formulas.
\begin{enumerate}[label=(\alph*)]
    \item $\neg (\neg P \wedge \neg Q).$
    \item $(P \wedge Q) \vee (P \wedge \neg Q).$
    \item $\neg (P \wedge \neg Q) \vee (\neg P \wedge Q).$
\end{enumerate}

\textbf{Solution:}
\begin{enumerate}[label=(\alph*)]
    \item \textbf{$\bm{\neg (\neg P \wedge \neg Q) \equiv P \vee Q.}$}
        \begin{alignat*}{2}
            \neg (\neg P \wedge \neg Q) & \equiv \neg \neg P \vee \neg \neg Q && \quad \text{(DeMorgan's Law)} \\
            & \equiv P \vee Q && \quad \text{(Double Negation Law)}
        \end{alignat*}

    \item \textbf{$\bm{(P \wedge Q) \vee (P \wedge \neg Q) \equiv P.}$}
        \begin{alignat*}{2}
            (P \wedge Q) \vee (P \wedge \neg Q) & \equiv ((P \wedge Q) \vee P) \wedge ((P \wedge Q) \vee \neg Q) && \quad \text{(Distributive Law)}\\
            &\equiv P \wedge ((P \wedge Q) \vee \neg Q) && \quad \text{(Absorption Law)} \\
            &\equiv P \wedge [(P \vee \neg Q) \wedge (Q \vee \neg Q)] && \quad \text{(Distributive Law)} \\
            &\equiv P \wedge [(P \vee \neg Q) \wedge \text{Tautology}] && \quad \text{(Definition of Tautology)} \\
            &\equiv P \wedge (P \vee \neg Q]) && \quad \text{(Tautology Law)} \\
            &\equiv P && \quad \text{(Absorption Law)}
        \end{alignat*}

    \item \textbf{$\bm{\neg (P \wedge \neg Q) \vee (\neg P \wedge Q) \equiv \neg P \vee Q.}$}
        \begin{alignat*}{2}
            \neg (P \wedge \neg Q) \vee (\neg P \wedge Q) &\equiv (\neg P \vee \neg \neg Q) \vee (\neg P \wedge Q) && \quad \text{(DeMorgan's Law)} \\
            &\equiv (\neg P \vee Q) \vee (\neg P \wedge Q) && \quad \text{(Double Negation Law)} \\ 
            &\equiv [(\neg P \vee Q) \vee \neg P] \wedge [(\neg P \vee Q) \vee Q)] && \quad \text{(Distributive Law)} \\ 
            &\equiv [\neg P \vee Q \vee \neg P] \wedge [\neg P \vee Q \vee Q] && \quad \text{(Associative Law)} \\ 
            &\equiv [\neg P \vee \neg P \vee Q] \wedge [\neg P \vee Q \vee Q] && \quad \text{(Commutative Law)} \\ 
            &\equiv [(\neg P \vee \neg P) \vee Q] \wedge [\neg P \vee (Q \vee Q)] && \quad \text{(Associative Law)} \\ 
            &\equiv (\neg P \vee Q) \wedge (\neg P \vee Q) && \quad \text{(Idempotent Law)} \\ 
            &\equiv \neg P \vee Q && \quad \text{(Idempotent Law)} \\ 
        \end{alignat*}
\end{enumerate}

\pagebreak