Use the first DeMorgan's Law and the double negation law to derive the second DeMorgan's Law.

\textbf{Solution:} The first DeMorgan's Law states $\neg (P \wedge Q) \equiv \neg P \vee \neg Q$. Now, consider the following:

\begin{alignat*}{2}
    P \vee Q & \equiv \neg (\neg P  \wedge \neg Q) \quad && \text{(First DeMorgan's Law)} \\
    \neg (P \vee Q) & \equiv \neg \neg (\neg P  \wedge \neg Q) \quad && \text{(Negate Both Sides)} \\
    \neg (P \vee Q) & \equiv \neg P  \wedge \neg Q \quad && \text{(Double Negation Law)}\\
\end{alignat*}

Thus, we have derived the second DeMorgan's Law using only the first DeMorgan's Law and the double negation law.

\pagebreak